OpenvmFv/Spec/SHIFTIOP/srai.lean
@@ -1,22 +1,22 @@
-import OpenvmFv.Spec.RTYPE.local
+import OpenvmFv.Spec.SHIFTIOP.local
 import OpenvmFv.Spec.rX_bits
 
 namespace PureSpec
 
-  structure SllInput where
-    -- operands
+  structure SraiInput where
+    -- opersras
     r1_val : BitVec 32
-    r2_val : BitVec 32
+    imm : BitVec 6
     rd : Fin 32
     -- registers
     PC : BitVec 32
 
-  structure SllOutput where
+  structure SraiOutput where
     -- registers
     nextPC : BitVec 32
     rd : Option (Finset.Icc 1 31 × BitVec 32)
 
-  def execute_RTYPE_sll_pure (input : SllInput) : SllOutput := {
+  def execute_SHIFTIOP_srai_pure (input : SraiInput) : SraiOutput := {
     nextPC := input.PC + 4#32
     rd := if h: input.rd = 0
       then .none
@@ -25,28 +25,28 @@ namespace PureSpec
           input.rd.val,
           by apply Finset.mem_Icc.mpr; omega
         ⟩,
-        input.r1_val <<< (input.r2_val.toNat % 32)
+        input.r1_val.sshiftRight (input.imm % 32).toNat
       )
-    : SllOutput
+    : SraiOutput
   }
 
-  lemma execute_RTYPE_sll_pure_equiv
-    (sll_input : SllInput)
-    (r1 r2 rd: regidx)
-    (h_input_r1: read_xreg (regidx_to_fin r1) state = EStateM.Result.ok (sll_input.r1_val) state)
-    (h_input_r2: read_xreg (regidx_to_fin r2) state = EStateM.Result.ok (sll_input.r2_val) state)
-    (h_input_rd: sll_input.rd = regidx_to_fin rd)
-    (h_input_pc: state.regs.get? Register.PC = .some sll_input.PC)
+  lemma execute_SHIFTIOP_srai_pure_equiv
+    (srai_input : SraiInput)
+    (r1 rd: regidx)
+    (h_input_r1: read_xreg (regidx_to_fin r1) state = EStateM.Result.ok (srai_input.r1_val) state)
+    (h_input_imm: srai_input.imm = imm)
+    (h_input_rd: srai_input.rd = regidx_to_fin rd)
+    (h_input_pc: state.regs.get? Register.PC = .some srai_input.PC)
   :
     (
       do
         Sail.writeReg Register.nextPC (Sail.BitVec.addInt (← Sail.readReg Register.PC) 4)
-        LeanRV32D.Functions.execute (instruction.RTYPE (r2, r1, rd, rop.SLL))
+        LeanRV32D.Functions.execute (instruction.SHIFTIOP (imm, r1, rd, sop.SRAI))
     ) state =
-    let sll_output := execute_RTYPE_sll_pure sll_input
+    let srai_output := execute_SHIFTIOP_srai_pure srai_input
     (do
-      Sail.writeReg Register.nextPC sll_output.nextPC
-      match sll_output.rd with
+      Sail.writeReg Register.nextPC srai_output.nextPC
+      match srai_output.rd with
         | .some (rd, rd_val) => write_xreg rd rd_val
         | .none => pure ()
       pure (ExecutionResult.Retire_Success ())
@@ -68,19 +68,16 @@ namespace PureSpec
     simp [this]
 
     simp [
-      ←Local.execute_RTYPE_equiv,
-      Local.execute_RTYPE.eq_def,
+      ←Local.execute_SHIFTIOP_equiv,
+      Local.execute_SHIFTIOP.eq_def,
       bind, EStateM.instMonad, EStateM.bind
     ]
 
     rewrite [rX_read_xreg_equiv _ r1 (regidx_to_fin r1) (by simp [regidx_to_fin])]
     rewrite [read_xreg_write_reg_state_nextPC _ h_input_r1]
-    simp
-    rewrite [rX_read_xreg_equiv _ r2 (regidx_to_fin r2) (by simp [regidx_to_fin])]
-    rewrite [read_xreg_write_reg_state_nextPC _ h_input_r2]
     simp [EStateM.pure]
 
-    simp [execute_RTYPE_sll_pure]
+    simp [execute_SHIFTIOP_srai_pure]
 
     obtain ⟨rd⟩ := rd
     by_cases h_zero: rd = 0
@@ -100,10 +97,16 @@ namespace PureSpec
       ]
       simp [regidx_to_fin]
       rewrite [dite_cond_eq_false]
-      . simp [h_input_rd, regidx_to_fin]
-        simp [
-          Sail.shift_bits_left, Sail.BitVec.extractLsb, log2_xlen
+      . simp [
+          h_input_rd, regidx_to_fin, h_input_imm,
+          LeanRV32D.Functions.shift_bits_right_arith,
+          LeanRV32D.Functions.shift_right_arith,
+          Sail.BitVec.extractLsb,
+          log2_xlen,
+          Local.sign_extend_equiv
         ]
+        congr
+        grind
       . simp [regidx_to_fin] at *
         omega
 
