OpenvmFv/Equivalence/ALU.lean
@@ -1,0 +1,770 @@
+import OpenvmFv.Spec.ALU
+
+import OpenvmFv.Spec.RTYPE.add
+import OpenvmFv.Spec.RTYPE.sub
+import OpenvmFv.Spec.RTYPE.xor
+import OpenvmFv.Spec.RTYPE.or
+import OpenvmFv.Spec.RTYPE.and
+
+import OpenvmFv.Spec.ITYPE.addi
+import OpenvmFv.Spec.ITYPE.andi
+import OpenvmFv.Spec.ITYPE.ori
+import OpenvmFv.Spec.ITYPE.xori
+
+set_option maxHeartbeats 1_000_000_000
+
+namespace Equivalence.ALU
+
+  structure ALU_instruction_fields where
+    is_valid : FBB
+    non_imm : FBB
+
+    pc : FBB
+    next_pc : FBB
+
+    opcode : FBB
+
+    prev_a_timestamp : FBB
+    a_timestamp : FBB
+    prev_b_timestamp : FBB
+    b_timestamp : FBB
+    prev_c_timestamp : FBB
+    c_timestamp : FBB
+    timestamp : FBB
+    next_timestamp : FBB
+
+    rs1_ptr : FBB
+    rs2_ptr : FBB
+    rd_ptr : FBB
+
+    prev_a : Vector FBB 4
+    a : Vector FBB 4
+    b : Vector FBB 4
+    c : Vector FBB 4
+
+    range_checked_vals : Vector FBB 6
+    bitwise_vals : Vector (Vector FBB 3) 5
+
+  def wrap_to_regidx (val : FBB) : Fin 32 :=
+    ⟨val % 32, by grind⟩
+
+  def AddInput_of_ALU_instruction_fields (row : ALU_instruction_fields) : PureSpec.AddInput := {
+    r1_val := BabyBear.toBV32 row.b
+    r2_val := BabyBear.toBV32 row.c
+    rd := wrap_to_regidx row.rd_ptr
+    PC := row.pc.toNat
+    : PureSpec.AddInput
+  }
+
+  def AddiInput_of_ALU_instruction_fields (row : ALU_instruction_fields) : PureSpec.AddiInput := {
+    r1_val := BabyBear.toBV32 row.b
+    imm := BitVec.ofNat 12 row.rs2_ptr.toNat
+    rd := wrap_to_regidx row.rd_ptr
+    PC := row.pc.toNat
+    : PureSpec.AddiInput
+  }
+
+  def SubInput_of_ALU_instruction_fields (row : ALU_instruction_fields) : PureSpec.SubInput := {
+    r1_val := BabyBear.toBV32 row.b
+    r2_val := BabyBear.toBV32 row.c
+    rd := wrap_to_regidx row.rd_ptr
+    PC := row.pc.toNat
+    : PureSpec.SubInput
+  }
+
+  def XorInput_of_ALU_instruction_fields (row : ALU_instruction_fields) : PureSpec.XorInput := {
+    r1_val := BabyBear.toBV32 row.b
+    r2_val := BabyBear.toBV32 row.c
+    rd := wrap_to_regidx row.rd_ptr
+    PC := row.pc.toNat
+    : PureSpec.XorInput
+  }
+
+  def XoriInput_of_ALU_instruction_fields (row : ALU_instruction_fields) : PureSpec.XoriInput := {
+    r1_val := BabyBear.toBV32 row.b
+    imm := BitVec.ofNat 12 row.rs2_ptr.toNat
+    rd := wrap_to_regidx row.rd_ptr
+    PC := row.pc.toNat
+    : PureSpec.XoriInput
+  }
+
+  def OrInput_of_ALU_instruction_fields (row : ALU_instruction_fields) : PureSpec.OrInput := {
+    r1_val := BabyBear.toBV32 row.b
+    r2_val := BabyBear.toBV32 row.c
+    rd := wrap_to_regidx row.rd_ptr
+    PC := row.pc.toNat
+    : PureSpec.OrInput
+  }
+
+  def OriInput_of_ALU_instruction_fields (row : ALU_instruction_fields) : PureSpec.OriInput := {
+    r1_val := BabyBear.toBV32 row.b
+    imm := BitVec.ofNat 12 row.rs2_ptr.toNat
+    rd := wrap_to_regidx row.rd_ptr
+    PC := row.pc.toNat
+    : PureSpec.OriInput
+  }
+
+  def AndInput_of_ALU_instruction_fields (row : ALU_instruction_fields) : PureSpec.AndInput := {
+    r1_val := BabyBear.toBV32 row.b
+    r2_val := BabyBear.toBV32 row.c
+    rd := wrap_to_regidx row.rd_ptr
+    PC := row.pc.toNat
+    : PureSpec.AndInput
+  }
+
+  def AndiInput_of_ALU_instruction_fields (row : ALU_instruction_fields) : PureSpec.AndiInput := {
+    r1_val := BabyBear.toBV32 row.b
+    imm := BitVec.ofNat 12 row.rs2_ptr.toNat
+    rd := wrap_to_regidx row.rd_ptr
+    PC := row.pc.toNat
+    : PureSpec.AndiInput
+  }
+
+  def AddOutput_matches_ALU_instruction_fields (row : ALU_instruction_fields) (add_output : PureSpec.AddOutput) : Prop :=
+    BabyBear.isU32 row.b ∧
+    BabyBear.isU32 row.c ∧
+    add_output.nextPC = row.next_pc.toNat ∧
+    match add_output.rd with
+      | .none => row.a = row.prev_a
+      | .some (rd, rd_val) =>
+        BabyBear.isU32 row.a ∧
+        BabyBear.toBV32 row.a = rd_val ∧
+        rd.1.toNat = row.rd_ptr.toNat
+
+  def AddiOutput_matches_ALU_instruction_fields (row : ALU_instruction_fields) (addi_output : PureSpec.AddiOutput) : Prop :=
+    BabyBear.isU32 row.b ∧
+    (BitVec.ofNat 12 (row.rs2_ptr)).signExtend 24 =
+    (BitVec.ofNat 24 (row.rs2_ptr)) ∧
+    addi_output.nextPC = row.next_pc.toNat ∧
+    match addi_output.rd with
+      | .none => row.a = row.prev_a
+      | .some (rd, rd_val) =>
+        BabyBear.isU32 row.a ∧
+        BabyBear.toBV32 row.a = rd_val ∧
+        rd.1.toNat = row.rd_ptr.toNat
+
+  def SubOutput_matches_ALU_instruction_fields (row : ALU_instruction_fields) (sub_output : PureSpec.SubOutput) : Prop :=
+    BabyBear.isU32 row.b ∧
+    BabyBear.isU32 row.c ∧
+    sub_output.nextPC = row.next_pc.toNat ∧
+    match sub_output.rd with
+      | .none => row.a = row.prev_a
+      | .some (rd, rd_val) =>
+        BabyBear.isU32 row.a ∧
+        BabyBear.toBV32 row.a = rd_val ∧
+        rd.1.toNat = row.rd_ptr.toNat
+
+  def XorOutput_matches_ALU_instruction_fields (row : ALU_instruction_fields) (xor_output : PureSpec.XorOutput) : Prop :=
+    BabyBear.isU32 row.b ∧
+    BabyBear.isU32 row.c ∧
+    xor_output.nextPC = row.next_pc.toNat ∧
+    match xor_output.rd with
+      | .none => row.a = row.prev_a
+      | .some (rd, rd_val) =>
+        BabyBear.isU32 row.a ∧
+        BabyBear.toBV32 row.a = rd_val ∧
+        rd.1.toNat = row.rd_ptr.toNat
+
+  def XoriOutput_matches_ALU_instruction_fields (row : ALU_instruction_fields) (xori_output : PureSpec.XoriOutput) : Prop :=
+    BabyBear.isU32 row.b ∧
+    (BitVec.ofNat 12 (row.rs2_ptr)).signExtend 24 =
+    (BitVec.ofNat 24 (row.rs2_ptr)) ∧
+    xori_output.nextPC = row.next_pc.toNat ∧
+    match xori_output.rd with
+      | .none => row.a = row.prev_a
+      | .some (rd, rd_val) =>
+        BabyBear.isU32 row.a ∧
+        BabyBear.toBV32 row.a = rd_val ∧
+        rd.1.toNat = row.rd_ptr.toNat
+
+  def OrOutput_matches_ALU_instruction_fields (row : ALU_instruction_fields) (or_output : PureSpec.OrOutput) : Prop :=
+    BabyBear.isU32 row.b ∧
+    BabyBear.isU32 row.c ∧
+    or_output.nextPC = row.next_pc.toNat ∧
+    match or_output.rd with
+      | .none => row.a = row.prev_a
+      | .some (rd, rd_val) =>
+        BabyBear.isU32 row.a ∧
+        BabyBear.toBV32 row.a = rd_val ∧
+        rd.1.toNat = row.rd_ptr.toNat
+
+  def OriOutput_matches_ALU_instruction_fields (row : ALU_instruction_fields) (ori_output : PureSpec.OriOutput) : Prop :=
+    BabyBear.isU32 row.b ∧
+    (BitVec.ofNat 12 (row.rs2_ptr)).signExtend 24 =
+    (BitVec.ofNat 24 (row.rs2_ptr)) ∧
+    ori_output.nextPC = row.next_pc.toNat ∧
+    match ori_output.rd with
+      | .none => row.a = row.prev_a
+      | .some (rd, rd_val) =>
+        BabyBear.isU32 row.a ∧
+        BabyBear.toBV32 row.a = rd_val ∧
+        rd.1.toNat = row.rd_ptr.toNat
+
+  def AndOutput_matches_ALU_instruction_fields (row : ALU_instruction_fields) (and_output : PureSpec.AndOutput) : Prop :=
+    BabyBear.isU32 row.b ∧
+    BabyBear.isU32 row.c ∧
+    and_output.nextPC = row.next_pc.toNat ∧
+    match and_output.rd with
+      | .none => row.a = row.prev_a
+      | .some (rd, rd_val) =>
+        BabyBear.isU32 row.a ∧
+        BabyBear.toBV32 row.a = rd_val ∧
+        rd.1.toNat = row.rd_ptr.toNat
+
+  def AndiOutput_matches_ALU_instruction_fields (row : ALU_instruction_fields) (andi_output : PureSpec.AndiOutput) : Prop :=
+    BabyBear.isU32 row.b ∧
+    (BitVec.ofNat 12 (row.rs2_ptr)).signExtend 24 =
+    (BitVec.ofNat 24 (row.rs2_ptr)) ∧
+    andi_output.nextPC = row.next_pc.toNat ∧
+    match andi_output.rd with
+      | .none => row.a = row.prev_a
+      | .some (rd, rd_val) =>
+        BabyBear.isU32 row.a ∧
+        BabyBear.toBV32 row.a = rd_val ∧
+        rd.1.toNat = row.rd_ptr.toNat
+
+  def ALU_instruction_fields.spec (row : ALU_instruction_fields) : Prop :=
+    row.is_valid = 1 → (
+      (row.non_imm = 0 ∨ row.non_imm = 1) ∧
+      row.opcode ∈ Finset.Icc 512 516 ∧
+      (row.non_imm = 1 → (
+        (row.opcode = 512 →
+          AddOutput_matches_ALU_instruction_fields
+            row
+            (PureSpec.execute_RTYPE_add_pure (AddInput_of_ALU_instruction_fields row))
+        ) ∧
+        (row.opcode = 513 →
+          SubOutput_matches_ALU_instruction_fields
+            row
+            (PureSpec.execute_RTYPE_sub_pure (SubInput_of_ALU_instruction_fields row))
+        ) ∧
+        (row.opcode = 514 →
+          XorOutput_matches_ALU_instruction_fields
+            row
+            (PureSpec.execute_RTYPE_xor_pure (XorInput_of_ALU_instruction_fields row))
+        ) ∧
+        (row.opcode = 515 →
+          OrOutput_matches_ALU_instruction_fields
+            row
+            (PureSpec.execute_RTYPE_or_pure (OrInput_of_ALU_instruction_fields row))
+        ) ∧
+        (row.opcode = 516 →
+          AndOutput_matches_ALU_instruction_fields
+            row
+            (PureSpec.execute_RTYPE_and_pure (AndInput_of_ALU_instruction_fields row))
+        )
+      )) ∧
+      (row.non_imm = 0 → (
+        (row.opcode = 512 →
+          AddiOutput_matches_ALU_instruction_fields
+            row
+            (PureSpec.execute_ITYPE_addi_pure (AddiInput_of_ALU_instruction_fields row))
+        ) ∧
+        (row.opcode ≠ 513) ∧
+        (row.opcode = 514 →
+          XoriOutput_matches_ALU_instruction_fields
+            row
+            (PureSpec.execute_ITYPE_xori_pure (XoriInput_of_ALU_instruction_fields row))
+        ) ∧
+        (row.opcode = 515 →
+          OriOutput_matches_ALU_instruction_fields
+            row
+            (PureSpec.execute_ITYPE_ori_pure (OriInput_of_ALU_instruction_fields row))
+        ) ∧
+        (row.opcode = 516 →
+          AndiOutput_matches_ALU_instruction_fields
+            row
+            (PureSpec.execute_ITYPE_andi_pure (AndiInput_of_ALU_instruction_fields row))
+        )
+      ))
+    )
+
+  def ALU_instruction_fields.execution (row : ALU_instruction_fields) : List (FBB × List FBB) := [
+    (-row.is_valid, [row.pc, row.timestamp]),
+    (row.is_valid, [row.next_pc, row.next_timestamp])
+  ]
+
+  def ALU_instruction_fields.memory (row : ALU_instruction_fields) : List (FBB × List FBB) := [
+    (-row.is_valid, [1, row.rs1_ptr, row.b[0], row.b[1], row.b[2], row.b[3], row.prev_b_timestamp]),
+    ( row.is_valid, [1, row.rs1_ptr, row.b[0], row.b[1], row.b[2], row.b[3], row.b_timestamp]),
+    (-row.non_imm, [row.non_imm, row.rs2_ptr, row.c[0], row.c[1], row.c[2], row.c[3], row.prev_c_timestamp]),
+    ( row.non_imm, [row.non_imm, row.rs2_ptr, row.c[0], row.c[1], row.c[2], row.c[3], row.c_timestamp]),
+    (-row.is_valid, [1, row.rd_ptr, row.prev_a[0], row.prev_a[1], row.prev_a[2], row.prev_a[3], row.prev_a_timestamp]),
+    ( row.is_valid, [1, row.rd_ptr, row.a[0], row.a[1], row.a[2], row.a[3], row.a_timestamp]),
+  ]
+
+  def ALU_instruction_fields.range_checks (row : ALU_instruction_fields) : List (FBB × List FBB) := [
+    (row.is_valid, [row.range_checked_vals[0], 17]),
+    (row.is_valid, [row.range_checked_vals[1], 12]),
+    (row.non_imm, [row.range_checked_vals[2], 17]),
+    (row.non_imm, [row.range_checked_vals[3], 12]),
+    (row.is_valid, [row.range_checked_vals[4], 17]),
+    (row.is_valid, [row.range_checked_vals[5], 12]),
+  ]
+
+  def ALU_instruction_fields.read_instruction (row : ALU_instruction_fields) : List (FBB × List FBB) := [
+    (row.is_valid, [row.pc, row.opcode, row.rd_ptr, row.rs1_ptr, row.rs2_ptr, 1, row.non_imm, 0, 0])
+  ]
+
+  def ALU_instruction_fields.bitwise (row : ALU_instruction_fields) : List (FBB × List FBB) := [
+    (row.is_valid, [row.bitwise_vals[0][0], row.bitwise_vals[0][1], row.bitwise_vals[0][2], 1]),
+    (row.is_valid, [row.bitwise_vals[1][0], row.bitwise_vals[1][1], row.bitwise_vals[1][2], 1]),
+    (row.is_valid, [row.bitwise_vals[2][0], row.bitwise_vals[2][1], row.bitwise_vals[2][2], 1]),
+    (row.is_valid, [row.bitwise_vals[3][0], row.bitwise_vals[3][1], row.bitwise_vals[3][2], 1]),
+    (row.is_valid - row.non_imm, [row.bitwise_vals[4][0], row.bitwise_vals[4][1], row.bitwise_vals[4][2], 0]),
+  ]
+
+  def bus_from_instruction_fields (rows : List ALU_instruction_fields) : ℕ → List (FBB × List FBB) :=
+    λ index =>
+      if index = ExecutionBus then            rows.flatMap ALU_instruction_fields.execution
+      else if index = MemoryBus then          rows.flatMap ALU_instruction_fields.memory
+      else if index = RangeCheckerBus then    rows.flatMap ALU_instruction_fields.range_checks
+      else if index = ReadInstructionBus then rows.flatMap ALU_instruction_fields.read_instruction
+      else if index = BitwiseBus then         rows.flatMap ALU_instruction_fields.bitwise
+      else []
+
+  def allHold_allRows [Field ExtF] (air : Valid_VmAirWrapper_alu FBB ExtF) : Prop :=
+    ∀ row : (Fin (air.last_row + 1)), VmAirWrapper_alu.constraints.allHold air row.1 (by grind)
+
+  def get_instruction_fields (air : Valid_VmAirWrapper_alu FBB ExtF) : List ALU_instruction_fields :=
+    (List.range (air.last_row + 1)).map (λ row => {
+      is_valid := air.core.is_valid row 0
+      non_imm := air.adapter.rs2_as row 0
+      pc := air.adapter.from_state.pc row 0
+      next_pc := air.adapter.from_state.pc row 0 + 4
+      opcode := (air.core.ctx row 0).instruction.opcode
+      prev_a_timestamp := air.adapter.writes_aux.base.prev_timestamp row 0
+      a_timestamp := air.adapter.from_state.timestamp row 0 + 2
+      prev_b_timestamp := air.adapter.reads_aux_0.base.prev_timestamp row 0
+      b_timestamp := air.adapter.from_state.timestamp row 0
+      prev_c_timestamp := air.adapter.reads_aux_1.base.prev_timestamp row 0
+      c_timestamp := air.adapter.from_state.timestamp row 0 + 1
+      timestamp := air.adapter.from_state.timestamp row 0
+      next_timestamp := air.adapter.from_state.timestamp row 0 + 3
+      rs1_ptr := air.adapter.rs1_ptr row 0
+      rs2_ptr := air.adapter.rs2 row 0
+      rd_ptr := air.adapter.rd_ptr row 0
+      prev_a := #v[air.adapter.writes_aux.prev_data_0 row 0,
+                   air.adapter.writes_aux.prev_data_1 row 0,
+                   air.adapter.writes_aux.prev_data_2 row 0,
+                   air.adapter.writes_aux.prev_data_3 row 0]
+      a := #v[air.core.a_0 row 0, air.core.a_1 row 0, air.core.a_2 row 0, air.core.a_3 row 0]
+      b := #v[air.core.b_0 row 0, air.core.b_1 row 0, air.core.b_2 row 0, air.core.b_3 row 0]
+      c := #v[air.core.c_0 row 0, air.core.c_1 row 0, air.core.c_2 row 0, air.core.c_3 row 0]
+      range_checked_vals :=
+        #v[air.adapter.reads_aux_0.base.timestamp_lt_aux.lower_decomp_0 row 0,
+           air.adapter.reads_aux_0.base.timestamp_lt_aux.lower_decomp_1 row 0,
+           air.adapter.reads_aux_1.base.timestamp_lt_aux.lower_decomp_0 row 0,
+           air.adapter.reads_aux_1.base.timestamp_lt_aux.lower_decomp_1 row 0,
+           air.adapter.writes_aux.base.timestamp_lt_aux.lower_decomp_0 row 0,
+           air.adapter.writes_aux.base.timestamp_lt_aux.lower_decomp_1 row 0]
+      bitwise_vals :=
+        #v[
+          #v[air.core.x_0 row 0, air.core.y_0 row 0, air.core.x_xor_y_0 row 0],
+          #v[air.core.x_1 row 0, air.core.y_1 row 0, air.core.x_xor_y_1 row 0],
+          #v[air.core.x_2 row 0, air.core.y_2 row 0, air.core.x_xor_y_2 row 0],
+          #v[air.core.x_3 row 0, air.core.y_3 row 0, air.core.x_xor_y_3 row 0],
+          #v[air.core.c_0 row 0, air.core.c_1 row 0, 0]
+        ]
+      : ALU_instruction_fields
+    })
+
+  theorem alu_spec [Field ExtF]
+    (air : Valid_VmAirWrapper_alu FBB ExtF)
+    (h_constraints : allHold_allRows air)
+    (h_bus_assumptions : ∀ row ≤ air.last_row, VmAirWrapper_alu.constraints.assumptionsPerRow air row)
+    (h_bus_wellformedness : ∀ row ≤ air.last_row, VmAirWrapper_alu.constraints.wf_propertiesToAssumePerRow air row)
+  :
+    ∃ instruction_fields_list : List ALU_instruction_fields,
+      air.buses = bus_from_instruction_fields instruction_fields_list ∧
+      instruction_fields_list.Forall ALU_instruction_fields.spec
+  := by
+    have h_neg_one : (2013265920 : FBB) = (-1 : FBB) := rfl
+
+    have h_interactions := VmAirWrapper_alu.constraints.constrain_interactions_of_extraction air (h_constraints 0).1
+    unfold allHold_allRows at h_constraints
+    use get_instruction_fields air
+    split_ands
+    . unfold VmAirWrapper_alu.constraints.constrain_interactions at h_interactions
+      rewrite [h_interactions]; clear h_interactions
+      unfold bus_from_instruction_fields ALU_instruction_fields.execution ALU_instruction_fields.memory ALU_instruction_fields.range_checks ALU_instruction_fields.read_instruction ALU_instruction_fields.bitwise
+      simp [
+        get_instruction_fields,
+        VmAirWrapper_alu_constraint_and_interaction_simplification
+      ]
+      unfold VmAirWrapper_alu.constraints.executionBus_row
+      unfold VmAirWrapper_alu.constraints.memoryBus_row
+      unfold VmAirWrapper_alu.constraints.rangeCheckerBus_row
+      unfold VmAirWrapper_alu.constraints.readInstructionBus_row
+      unfold VmAirWrapper_alu.constraints.bitwiseBus_row
+      funext index
+      by_cases h_index: index = ExecutionBus
+      . simp [h_index, List.flatMap_map]
+      by_cases h_index: index = MemoryBus
+      . simp [h_index, List.flatMap_map]
+        congr
+        funext row
+        congr
+        all_goals simp [h_neg_one]
+      by_cases h_index: index = RangeCheckerBus
+      . simp [h_index, List.flatMap_map]
+      by_cases h_index: index = ReadInstructionBus
+      . simp [h_index, List.flatMap_map]
+      by_cases h_index: index = BitwiseBus
+      . simp [h_index, List.flatMap_map]
+      . simp [*]
+    . apply List.forall_iff_forall_mem.mpr
+      intro instruction_fields h_instruction_fields
+      unfold ALU_instruction_fields.spec
+      simp [get_instruction_fields] at h_instruction_fields
+      obtain ⟨row, ⟨h_row_range, h_fields⟩⟩ := h_instruction_fields
+      rewrite [←h_fields]; clear h_fields
+      simp
+
+      intro h_is_valid
+
+      have ⟨
+        h_pc,
+        h_timestamp,
+        ⟨h_a0, h_a1, h_a2, h_a3, h_b0, h_b1, h_b2, h_b3, h_c0, h_c1, h_c2, h_c3⟩,
+        h_opcodes,
+        h_imm_binary,
+        h_imm_op_properties
+      ⟩ := ALU.ValidRows.essentials
+        ExtF
+        air
+        row
+        (by omega)
+        (h_constraints ⟨row, by omega⟩)
+        h_is_valid
+        (h_bus_assumptions row (by omega))
+        (h_bus_wellformedness row (by omega))
+      simp only [h_imm_binary, true_and]
+      clear h_imm_binary
+
+      -- discharge opcode range, leave non-imm specs and imm-specs respectively
+      split_ands <;> [grind; grind; skip; skip]
+
+      . intro h_non_imm
+        have non_imm_spec := ALU.ValidRows.spec_base_ALU_non_imm
+          ExtF
+          air
+          row
+          (by omega)
+          (h_constraints ⟨row, by omega⟩)
+          h_is_valid
+          (h_bus_wellformedness row (by omega))
+
+        dsimp only at *
+
+        split_ands
+        . intro h_opcode
+          simp [AddOutput_matches_ALU_instruction_fields]
+          split_ands <;>
+          [ assumption; assumption; assumption; assumption;
+            assumption; assumption; assumption; assumption;
+            skip; skip ]
+          . simp [AddInput_of_ALU_instruction_fields, BabyBear.toBV32, PureSpec.execute_RTYPE_add_pure]
+            simp [← BitVec.toNat_inj]
+            omega
+          . simp [AddInput_of_ALU_instruction_fields, BabyBear.toBV32, PureSpec.execute_RTYPE_add_pure]
+            rewrite [dite_cond_eq_false]
+            . simp
+              split_ands <;>
+              [ assumption; assumption; assumption; assumption; skip; skip ]
+              . specialize non_imm_spec h_non_imm
+                unfold execute_RTYPE_pure at non_imm_spec
+                simp only [h_opcode, ALU.ValidRows.rop_of_ALU_opcode] at non_imm_spec
+                dsimp at non_imm_spec
+                assumption
+              . simp [wrap_to_regidx]
+                specialize h_bus_wellformedness row (by omega)
+                simp [VmAirWrapper_alu_constraint_and_interaction_simplification,
+                      Interaction.ReadInstructionBusEntry.operand_properties] at h_bus_wellformedness
+                omega
+            . simp [wrap_to_regidx]
+              specialize h_bus_wellformedness row (by omega)
+              simp [VmAirWrapper_alu_constraint_and_interaction_simplification,
+                    Interaction.ReadInstructionBusEntry.operand_properties] at h_bus_wellformedness
+              omega
+        . intro h_opcode
+          simp [SubOutput_matches_ALU_instruction_fields]
+          split_ands <;>
+          [ assumption; assumption; assumption; assumption;
+            assumption; assumption; assumption; assumption;
+            skip; skip ]
+          . simp [SubInput_of_ALU_instruction_fields, BabyBear.toBV32, PureSpec.execute_RTYPE_sub_pure]
+            simp [← BitVec.toNat_inj]
+            omega
+          . simp [SubInput_of_ALU_instruction_fields, BabyBear.toBV32, PureSpec.execute_RTYPE_sub_pure]
+            rewrite [dite_cond_eq_false]
+            . simp
+              split_ands <;>
+              [ assumption; assumption; assumption; assumption; skip; skip ]
+              . specialize non_imm_spec h_non_imm
+                unfold execute_RTYPE_pure at non_imm_spec
+                simp only [h_opcode, ALU.ValidRows.rop_of_ALU_opcode] at non_imm_spec
+                dsimp at non_imm_spec
+                assumption
+              . simp [wrap_to_regidx]
+                specialize h_bus_wellformedness row (by omega)
+                simp [VmAirWrapper_alu_constraint_and_interaction_simplification,
+                      Interaction.ReadInstructionBusEntry.operand_properties] at h_bus_wellformedness
+                omega
+            . simp [wrap_to_regidx]
+              specialize h_bus_wellformedness row (by omega)
+              simp [VmAirWrapper_alu_constraint_and_interaction_simplification,
+                    Interaction.ReadInstructionBusEntry.operand_properties] at h_bus_wellformedness
+              omega
+        . intro h_opcode
+          simp [XorOutput_matches_ALU_instruction_fields]
+          split_ands <;>
+          [ assumption; assumption; assumption; assumption;
+            assumption; assumption; assumption; assumption;
+            skip; skip ]
+          . simp [XorInput_of_ALU_instruction_fields, BabyBear.toBV32, PureSpec.execute_RTYPE_xor_pure]
+            simp [← BitVec.toNat_inj]
+            omega
+          . simp [XorInput_of_ALU_instruction_fields, BabyBear.toBV32, PureSpec.execute_RTYPE_xor_pure]
+            rewrite [dite_cond_eq_false]
+            . simp
+              split_ands <;>
+              [ assumption; assumption; assumption; assumption; skip; skip ]
+              . specialize non_imm_spec h_non_imm
+                unfold execute_RTYPE_pure at non_imm_spec
+                simp only [h_opcode, ALU.ValidRows.rop_of_ALU_opcode] at non_imm_spec
+                dsimp at non_imm_spec
+                assumption
+              . simp [wrap_to_regidx]
+                specialize h_bus_wellformedness row (by omega)
+                simp [VmAirWrapper_alu_constraint_and_interaction_simplification,
+                      Interaction.ReadInstructionBusEntry.operand_properties] at h_bus_wellformedness
+                omega
+            . simp [wrap_to_regidx]
+              specialize h_bus_wellformedness row (by omega)
+              simp [VmAirWrapper_alu_constraint_and_interaction_simplification,
+                    Interaction.ReadInstructionBusEntry.operand_properties] at h_bus_wellformedness
+              omega
+        . intro h_opcode
+          simp [OrOutput_matches_ALU_instruction_fields]
+          split_ands <;>
+          [ assumption; assumption; assumption; assumption;
+            assumption; assumption; assumption; assumption;
+            skip; skip ]
+          . simp [OrInput_of_ALU_instruction_fields, BabyBear.toBV32, PureSpec.execute_RTYPE_or_pure]
+            simp [← BitVec.toNat_inj]
+            omega
+          . simp [OrInput_of_ALU_instruction_fields, BabyBear.toBV32, PureSpec.execute_RTYPE_or_pure]
+            rewrite [dite_cond_eq_false]
+            . simp
+              split_ands <;>
+              [ assumption; assumption; assumption; assumption; skip; skip ]
+              . specialize non_imm_spec h_non_imm
+                unfold execute_RTYPE_pure at non_imm_spec
+                simp only [h_opcode, ALU.ValidRows.rop_of_ALU_opcode] at non_imm_spec
+                dsimp at non_imm_spec
+                assumption
+              . simp [wrap_to_regidx]
+                specialize h_bus_wellformedness row (by omega)
+                simp [VmAirWrapper_alu_constraint_and_interaction_simplification,
+                      Interaction.ReadInstructionBusEntry.operand_properties] at h_bus_wellformedness
+                omega
+            . simp [wrap_to_regidx]
+              specialize h_bus_wellformedness row (by omega)
+              simp [VmAirWrapper_alu_constraint_and_interaction_simplification,
+                    Interaction.ReadInstructionBusEntry.operand_properties] at h_bus_wellformedness
+              omega
+        . intro h_opcode
+          simp [AndOutput_matches_ALU_instruction_fields]
+          split_ands <;>
+          [ assumption; assumption; assumption; assumption;
+            assumption; assumption; assumption; assumption;
+            skip; skip ]
+          . simp [AndInput_of_ALU_instruction_fields, BabyBear.toBV32, PureSpec.execute_RTYPE_and_pure]
+            simp [← BitVec.toNat_inj]
+            omega
+          . simp [AndInput_of_ALU_instruction_fields, BabyBear.toBV32, PureSpec.execute_RTYPE_and_pure]
+            rewrite [dite_cond_eq_false]
+            . simp
+              split_ands <;>
+              [ assumption; assumption; assumption; assumption; skip; skip ]
+              . specialize non_imm_spec h_non_imm
+                unfold execute_RTYPE_pure at non_imm_spec
+                simp only [h_opcode, ALU.ValidRows.rop_of_ALU_opcode] at non_imm_spec
+                dsimp at non_imm_spec
+                assumption
+              . simp [wrap_to_regidx]
+                specialize h_bus_wellformedness row (by omega)
+                simp [VmAirWrapper_alu_constraint_and_interaction_simplification,
+                      Interaction.ReadInstructionBusEntry.operand_properties] at h_bus_wellformedness
+                omega
+            . simp [wrap_to_regidx]
+              specialize h_bus_wellformedness row (by omega)
+              simp [VmAirWrapper_alu_constraint_and_interaction_simplification,
+                    Interaction.ReadInstructionBusEntry.operand_properties] at h_bus_wellformedness
+              omega
+      . intro h_imm
+        have imm_spec := ALU.ValidRows.spec_base_ALU_imm
+          ExtF
+          air
+          row
+          (by omega)
+          (h_constraints ⟨row, by omega⟩)
+          h_is_valid
+          (h_bus_assumptions row (by omega))
+          (h_bus_wellformedness row (by omega))
+          h_imm
+
+        dsimp only at *
+
+        split_ands
+
+        . intro h_opcode
+          simp [AddiOutput_matches_ALU_instruction_fields]
+          split_ands <;>
+          [ assumption; assumption; assumption; assumption;
+            skip; skip; skip ]
+          . clear *-h_imm_op_properties h_imm
+            simp [h_imm] at h_imm_op_properties
+            have := @BitVec.toInt_signExtend 12 24 (BitVec.ofNat 12 ↑(air.adapter.rs2 row 0))
+            apply BitVec.eq_of_toInt_eq
+            rewrite [this]
+            simp
+            have := h_imm_op_properties.2.2.1
+            rewrite [this]
+            exact Int.bmod_eq_of_le (by grind) (by grind)
+          . simp [AddiInput_of_ALU_instruction_fields, BabyBear.toBV32, PureSpec.execute_ITYPE_addi_pure]
+            simp [← BitVec.toNat_inj]
+            omega
+          . simp [AddiInput_of_ALU_instruction_fields, BabyBear.toBV32, PureSpec.execute_ITYPE_addi_pure]
+            rewrite [dite_cond_eq_false]
+            . simp
+              split_ands <;>
+              [ assumption; assumption; assumption; assumption; skip; skip ]
+              . unfold execute_ITYPE_pure at imm_spec
+                simp only [h_opcode, ALU.ValidRows.iop_of_ALU_opcode] at imm_spec
+                dsimp at imm_spec
+                assumption
+              . simp [wrap_to_regidx]
+                specialize h_bus_wellformedness row (by omega)
+                simp [VmAirWrapper_alu_constraint_and_interaction_simplification,
+                      Interaction.ReadInstructionBusEntry.operand_properties] at h_bus_wellformedness
+                omega
+            . simp [wrap_to_regidx]
+              specialize h_bus_wellformedness row (by omega)
+              simp [VmAirWrapper_alu_constraint_and_interaction_simplification,
+                    Interaction.ReadInstructionBusEntry.operand_properties] at h_bus_wellformedness
+              omega
+        . specialize h_imm_op_properties h_imm
+          clear *-h_imm_op_properties
+          grind
+        . intro h_opcode
+          simp [XoriOutput_matches_ALU_instruction_fields]
+          split_ands <;>
+          [ assumption; assumption; assumption; assumption;
+            skip; skip; skip ]
+          . clear *-h_imm_op_properties h_imm
+            simp [h_imm] at h_imm_op_properties
+            have := @BitVec.toInt_signExtend 12 24 (BitVec.ofNat 12 ↑(air.adapter.rs2 row 0))
+            apply BitVec.eq_of_toInt_eq
+            rewrite [this]
+            simp
+            have := h_imm_op_properties.2.2.1
+            rewrite [this]
+            exact Int.bmod_eq_of_le (by grind) (by grind)
+          . simp [XoriInput_of_ALU_instruction_fields, BabyBear.toBV32, PureSpec.execute_ITYPE_xori_pure]
+            simp [← BitVec.toNat_inj]
+            omega
+          . simp [XoriInput_of_ALU_instruction_fields, BabyBear.toBV32, PureSpec.execute_ITYPE_xori_pure]
+            rewrite [dite_cond_eq_false]
+            . simp
+              split_ands <;>
+              [ assumption; assumption; assumption; assumption; skip; skip ]
+              . unfold execute_ITYPE_pure at imm_spec
+                simp only [h_opcode, ALU.ValidRows.iop_of_ALU_opcode] at imm_spec
+                dsimp at imm_spec
+                assumption
+              . simp [wrap_to_regidx]
+                specialize h_bus_wellformedness row (by omega)
+                simp [VmAirWrapper_alu_constraint_and_interaction_simplification,
+                      Interaction.ReadInstructionBusEntry.operand_properties] at h_bus_wellformedness
+                omega
+            . simp [wrap_to_regidx]
+              specialize h_bus_wellformedness row (by omega)
+              simp [VmAirWrapper_alu_constraint_and_interaction_simplification,
+                    Interaction.ReadInstructionBusEntry.operand_properties] at h_bus_wellformedness
+              omega
+        . intro h_opcode
+          simp [OriOutput_matches_ALU_instruction_fields]
+          split_ands <;>
+          [ assumption; assumption; assumption; assumption;
+            skip; skip; skip ]
+          . clear *-h_imm_op_properties h_imm
+            simp [h_imm] at h_imm_op_properties
+            have := @BitVec.toInt_signExtend 12 24 (BitVec.ofNat 12 ↑(air.adapter.rs2 row 0))
+            apply BitVec.eq_of_toInt_eq
+            rewrite [this]
+            simp
+            have := h_imm_op_properties.2.2.1
+            rewrite [this]
+            exact Int.bmod_eq_of_le (by grind) (by grind)
+          . simp [OriInput_of_ALU_instruction_fields, BabyBear.toBV32, PureSpec.execute_ITYPE_ori_pure]
+            simp [← BitVec.toNat_inj]
+            omega
+          . simp [OriInput_of_ALU_instruction_fields, BabyBear.toBV32, PureSpec.execute_ITYPE_ori_pure]
+            rewrite [dite_cond_eq_false]
+            . simp
+              split_ands <;>
+              [ assumption; assumption; assumption; assumption; skip; skip ]
+              . unfold execute_ITYPE_pure at imm_spec
+                simp only [h_opcode, ALU.ValidRows.iop_of_ALU_opcode] at imm_spec
+                dsimp at imm_spec
+                assumption
+              . simp [wrap_to_regidx]
+                specialize h_bus_wellformedness row (by omega)
+                simp [VmAirWrapper_alu_constraint_and_interaction_simplification,
+                      Interaction.ReadInstructionBusEntry.operand_properties] at h_bus_wellformedness
+                omega
+            . simp [wrap_to_regidx]
+              specialize h_bus_wellformedness row (by omega)
+              simp [VmAirWrapper_alu_constraint_and_interaction_simplification,
+                    Interaction.ReadInstructionBusEntry.operand_properties] at h_bus_wellformedness
+              omega
+        . intro h_opcode
+          simp [AndiOutput_matches_ALU_instruction_fields]
+          split_ands <;>
+          [ assumption; assumption; assumption; assumption;
+            skip; skip; skip ]
+          . clear *-h_imm_op_properties h_imm
+            simp [h_imm] at h_imm_op_properties
+            have := @BitVec.toInt_signExtend 12 24 (BitVec.ofNat 12 ↑(air.adapter.rs2 row 0))
+            apply BitVec.eq_of_toInt_eq
+            rewrite [this]
+            simp
+            have := h_imm_op_properties.2.2.1
+            rewrite [this]
+            exact Int.bmod_eq_of_le (by grind) (by grind)
+          . simp [AndiInput_of_ALU_instruction_fields, BabyBear.toBV32, PureSpec.execute_ITYPE_andi_pure]
+            simp [← BitVec.toNat_inj]
+            omega
+          . simp [AndiInput_of_ALU_instruction_fields, BabyBear.toBV32, PureSpec.execute_ITYPE_andi_pure]
+            rewrite [dite_cond_eq_false]
+            . simp
+              split_ands <;>
+              [ assumption; assumption; assumption; assumption; skip; skip ]
+              . unfold execute_ITYPE_pure at imm_spec
+                simp only [h_opcode, ALU.ValidRows.iop_of_ALU_opcode] at imm_spec
+                dsimp at imm_spec
+                assumption
+              . simp [wrap_to_regidx]
+                specialize h_bus_wellformedness row (by omega)
+                simp [VmAirWrapper_alu_constraint_and_interaction_simplification,
+                      Interaction.ReadInstructionBusEntry.operand_properties] at h_bus_wellformedness
+                omega
+            . simp [wrap_to_regidx]
+              specialize h_bus_wellformedness row (by omega)
+              simp [VmAirWrapper_alu_constraint_and_interaction_simplification,
+                    Interaction.ReadInstructionBusEntry.operand_properties] at h_bus_wellformedness
+              omega
+
+end Equivalence.ALU
