OpenvmFv/Spec/RTYPE/srl.lean
@@ -1,106 +1,110 @@
 import OpenvmFv.Spec.RTYPE.local
 import OpenvmFv.Spec.rX_bits
 
-structure SrlInput where
-  -- operands
-  r1_val : BitVec 32
-  r2_val : BitVec 32
-  rd : Fin 32
-  -- registers
-  PC : BitVec 32
+namespace PureSpec
 
-structure SrlOutput where
-  -- registers
-  nextPC : BitVec 32
-  rd : Option (Finset.Icc 1 31 × BitVec 32)
+  structure SrlInput where
+    -- operands
+    r1_val : BitVec 32
+    r2_val : BitVec 32
+    rd : Fin 32
+    -- registers
+    PC : BitVec 32
 
-def execute_RTYPE_srl_pure (input : SrlInput) : SrlOutput := {
-  nextPC := input.PC + 4#32
-  rd := if h: input.rd = 0
-    then .none
-    else .some (
-      ⟨
-        input.rd.val,
-        by apply Finset.mem_Icc.mpr; omega
-      ⟩,
-      input.r2_val >>> (input.r1_val.toNat % 32)
-    )
-  : SrlOutput
-}
+  structure SrlOutput where
+    -- registers
+    nextPC : BitVec 32
+    rd : Option (Finset.Icc 1 31 × BitVec 32)
 
-lemma execute_RTYPE_srl_pure_equiv
-  (srl_input : SrlInput)
-  (r1 r2 rd: regidx)
-  (h_input_r1: read_xreg (regidx_to_fin r1) state = EStateM.Result.ok (srl_input.r1_val) state)
-  (h_input_r2: read_xreg (regidx_to_fin r2) state = EStateM.Result.ok (srl_input.r2_val) state)
-  (h_input_rd: srl_input.rd = regidx_to_fin rd)
-  (h_input_pc: state.regs.get? Register.PC = .some srl_input.PC)
-:
-  (
-    do
-      Sail.writeReg Register.nextPC (Sail.BitVec.addInt (← Sail.readReg Register.PC) 4)
-      LeanRV32D.Functions.execute (instruction.RTYPE (r1, r2, rd, rop.SRL))
-  ) state =
-  let srl_output := execute_RTYPE_srl_pure srl_input
-  (do
-    Sail.writeReg Register.nextPC srl_output.nextPC
-    match srl_output.rd with
-      | .some (rd, rd_val) => write_xreg rd rd_val
-      | .none => pure ()
-    pure (ExecutionResult.Retire_Success ())
-  ) state
-:= by
-  unfold bind Monad.toBind EStateM.instMonad
-  dsimp
-  unfold EStateM.bind
-  dsimp
+  def execute_RTYPE_srl_pure (input : SrlInput) : SrlOutput := {
+    nextPC := input.PC + 4#32
+    rd := if h: input.rd = 0
+      then .none
+      else .some (
+        ⟨
+          input.rd.val,
+          by apply Finset.mem_Icc.mpr; omega
+        ⟩,
+        input.r1_val >>> (input.r2_val.toNat % 32)
+      )
+    : SrlOutput
+  }
 
-  simp [
-    readReg_state h_input_pc,
-    writeReg_state_success,
-    ←Local.execute_equiv,
-    Local.execute.eq_def
-  ]
+  lemma execute_RTYPE_srl_pure_equiv
+    (srl_input : SrlInput)
+    (r1 r2 rd: regidx)
+    (h_input_r1: read_xreg (regidx_to_fin r1) state = EStateM.Result.ok (srl_input.r1_val) state)
+    (h_input_r2: read_xreg (regidx_to_fin r2) state = EStateM.Result.ok (srl_input.r2_val) state)
+    (h_input_rd: srl_input.rd = regidx_to_fin rd)
+    (h_input_pc: state.regs.get? Register.PC = .some srl_input.PC)
+  :
+    (
+      do
+        Sail.writeReg Register.nextPC (Sail.BitVec.addInt (← Sail.readReg Register.PC) 4)
+        LeanRV32D.Functions.execute (instruction.RTYPE (r2, r1, rd, rop.SRL))
+    ) state =
+    let srl_output := execute_RTYPE_srl_pure srl_input
+    (do
+      Sail.writeReg Register.nextPC srl_output.nextPC
+      match srl_output.rd with
+        | .some (rd, rd_val) => write_xreg rd rd_val
+        | .none => pure ()
+      pure (ExecutionResult.Retire_Success ())
+    ) state
+  := by
+    unfold bind Monad.toBind EStateM.instMonad
+    dsimp
+    unfold EStateM.bind
+    dsimp
 
-  have (x : BitVec 32) : Sail.BitVec.addInt x 4 = x + 4 := rfl
-  simp [this]
-
-  simp [
-    ←Local.execute_RTYPE_equiv,
-    Local.execute_RTYPE.eq_def,
-    bind, EStateM.instMonad, EStateM.bind
-  ]
-
-  rewrite [rX_read_xreg_equiv _ r2 (regidx_to_fin r2) (by simp [regidx_to_fin])]
-  rewrite [read_xreg_write_reg_state_nextPC _ h_input_r2]
-  simp
-  rewrite [rX_read_xreg_equiv _ r1 (regidx_to_fin r1) (by simp [regidx_to_fin])]
-  rewrite [read_xreg_write_reg_state_nextPC _ h_input_r1]
-  simp [EStateM.pure]
-
-  simp [execute_RTYPE_srl_pure]
-
-  obtain ⟨rd⟩ := rd
-  by_cases h_zero: rd = 0
-  . rewrite [h_zero, wX_write_xreg_0_equiv]
-    simp
-    rewrite [dite_cond_eq_true]
-    . simp
-    . simp [h_input_rd, h_zero, regidx_to_fin]
-  . have h_inc := regidx_non_zero h_zero
-    apply Finset.mem_Icc.mp at h_inc
-    obtain ⟨h_low, h_high⟩ := h_inc
-    rewrite [
-      wX_write_xreg_equiv _ _
-        (regidx.Regidx rd)
-        ⟨(regidx_to_fin (regidx.Regidx rd)).val, Finset.mem_Icc.mpr ⟨h_low, h_high⟩⟩
-        (by simp [regidx_to_fin])
+    simp [
+      readReg_state h_input_pc,
+      writeReg_state_success,
+      ←Local.execute_equiv,
+      Local.execute.eq_def
     ]
-    simp [regidx_to_fin]
-    rewrite [dite_cond_eq_false]
-    . simp [h_input_rd, regidx_to_fin]
-      simp [
-        Sail.shift_bits_right, Sail.BitVec.extractLsb, log2_xlen
+
+    have (x : BitVec 32) : Sail.BitVec.addInt x 4 = x + 4 := rfl
+    simp [this]
+
+    simp [
+      ←Local.execute_RTYPE_equiv,
+      Local.execute_RTYPE.eq_def,
+      bind, EStateM.instMonad, EStateM.bind
+    ]
+
+    rewrite [rX_read_xreg_equiv _ r1 (regidx_to_fin r1) (by simp [regidx_to_fin])]
+    rewrite [read_xreg_write_reg_state_nextPC _ h_input_r1]
+    simp
+    rewrite [rX_read_xreg_equiv _ r2 (regidx_to_fin r2) (by simp [regidx_to_fin])]
+    rewrite [read_xreg_write_reg_state_nextPC _ h_input_r2]
+    simp [EStateM.pure]
+
+    simp [execute_RTYPE_srl_pure]
+
+    obtain ⟨rd⟩ := rd
+    by_cases h_zero: rd = 0
+    . rewrite [h_zero, wX_write_xreg_0_equiv]
+      simp
+      rewrite [dite_cond_eq_true]
+      . simp
+      . simp [h_input_rd, h_zero, regidx_to_fin]
+    . have h_inc := regidx_non_zero h_zero
+      apply Finset.mem_Icc.mp at h_inc
+      obtain ⟨h_low, h_high⟩ := h_inc
+      rewrite [
+        wX_write_xreg_equiv _ _
+          (regidx.Regidx rd)
+          ⟨(regidx_to_fin (regidx.Regidx rd)).val, Finset.mem_Icc.mpr ⟨h_low, h_high⟩⟩
+          (by simp [regidx_to_fin])
       ]
-    . simp [regidx_to_fin] at *
-      omega
+      simp [regidx_to_fin]
+      rewrite [dite_cond_eq_false]
+      . simp [h_input_rd, regidx_to_fin]
+        simp [
+          Sail.shift_bits_right, Sail.BitVec.extractLsb, log2_xlen
+        ]
+      . simp [regidx_to_fin] at *
+        omega
+
+end PureSpec
